Remove pf

src/lang/Local.v
@@ -27,8 +27,8 @@ Module ThreadEvent.
   | promise (loc:Loc.t) (from to:Time.t) (msg:Message.t) (kind:Memory.op_kind)
   | silent
   | read (loc:Loc.t) (ts:Time.t) (val:Const.t) (released:option View.t) (ord:Ordering.t)
-  | write (loc:Loc.t) (from to:Time.t) (val:Const.t) (released:option View.t) (ord:Ordering.t) (pf:bool)
-  | update (loc:Loc.t) (tsr tsw:Time.t) (valr valw:Const.t) (releasedr releasedw:option View.t) (ordr ordw:Ordering.t) (pf:bool)
+  | write (loc:Loc.t) (from to:Time.t) (val:Const.t) (released:option View.t) (ord:Ordering.t)
+  | update (loc:Loc.t) (tsr tsw:Time.t) (valr valw:Const.t) (releasedr releasedw:option View.t) (ordr ordw:Ordering.t)
   | fence (ordr ordw:Ordering.t)
   | syscall (e:Event.t)
   | failure
@@ -69,8 +69,8 @@ Module ThreadEvent.
     | promise _ _ _ _ _  => ProgramEvent.silent
     | silent => ProgramEvent.silent
     | read loc _ val _ ord => ProgramEvent.read loc val ord
-    | write loc _ _ val _ ord pf => ProgramEvent.write loc val ord pf
-    | update loc _ _ valr valw _ _ ordr ordw pf => ProgramEvent.update loc valr valw ordr ordw pf
+    | write loc _ _ val _ ord => ProgramEvent.write loc val ord
+    | update loc _ _ valr valw _ _ ordr ordw => ProgramEvent.update loc valr valw ordr ordw
     | fence ordr ordw => ProgramEvent.fence ordr ordw
     | syscall ev => ProgramEvent.syscall ev
     | failure => ProgramEvent.failure
@@ -92,22 +92,22 @@ Module ThreadEvent.
   Definition is_reading (e:t): option (Loc.t * Time.t * Const.t * option View.t * Ordering.t) :=
     match e with
     | read loc ts val released ord => Some (loc, ts, val, released, ord)
-    | update loc tsr _ valr _ releasedr _ ordr _ _ => Some (loc, tsr, valr, releasedr, ordr)
+    | update loc tsr _ valr _ releasedr _ ordr _ => Some (loc, tsr, valr, releasedr, ordr)
     | _ => None
     end.
 
-  Definition is_writing (e:t): option (Loc.t * Time.t * Time.t * Const.t * option View.t * Ordering.t * bool) :=
+  Definition is_writing (e:t): option (Loc.t * Time.t * Time.t * Const.t * option View.t * Ordering.t) :=
     match e with
-    | write loc from to val released ord pf => Some (loc, from, to, val, released, ord, pf)
-    | update loc tsr tsw _ valw _ releasedw _ ordw pf => Some (loc, tsr, tsw, valw, releasedw, ordw, pf)
+    | write loc from to val released ord => Some (loc, from, to, val, released, ord)
+    | update loc tsr tsw _ valw _ releasedw _ ordw => Some (loc, tsr, tsw, valw, releasedw, ordw)
     | _ => None
     end.
 
   Definition is_accessing (e:t): option (Loc.t * Time.t) :=
     match e with
     | read loc ts _ _ _ => Some (loc, ts)
-    | write loc _ ts _ _ _ _ => Some (loc, ts)
-    | update loc _ ts _ _ _ _ _ _ _ => Some (loc, ts)
+    | write loc _ ts _ _ _ => Some (loc, ts)
+    | update loc _ ts _ _ _ _ _ _ => Some (loc, ts)
     | _ => None
     end.
 
@@ -125,63 +125,6 @@ Module ThreadEvent.
     unfold is_accessing_loc.
     destruct e1, e2; ss; inv EVENT; ss.
   Qed.
-
-  (* TODO: unused *)
-
-  Inductive le: forall (lhs rhs:t), Prop :=
-  | le_promise
-      loc from to msg1 msg2 kind1 kind2
-      (LEREL: Message.le msg1 msg2):
-      le (promise loc from to msg1 kind1) (promise loc from to msg2 kind2)
-  | le_silent:
-      le silent silent
-  | le_read
-      loc ts val rel1 rel2 ord
-      (LEREL: View.opt_le rel1 rel2):
-      le (read loc ts val rel1 ord) (read loc ts val rel2 ord)
-  | le_write
-      loc from to val rel1 rel2 ord pf
-      (LEREL: View.opt_le rel1 rel2):
-      le (write loc from to val rel1 ord pf) (write loc from to val rel2 ord pf)
-  | le_update
-      loc tsr tsw valr valw relr1 relr2 relw1 relw2 ordr ordw pf
-      (LEREL: View.opt_le relr1 relr2)
-      (LEREL: View.opt_le relw1 relw2):
-      le (update loc tsr tsw valr valw relr1 relw1 ordr ordw pf)
-         (update loc tsr tsw valr valw relr2 relw2 ordr ordw pf)
-  | le_fence ordr ordw:
-      le (fence ordr ordw) (fence ordr ordw)
-  | le_syscall e:
-      le (syscall e) (syscall e)
-  | le_failure:
-      le failure failure
-  .
-  Hint Constructors le.
-
-  (* TODO: unused *)
-
-  (* Definition lift (ord0:Ordering.t) (e:t): t := *)
-  (*   match e with *)
-  (*   | promise loc from to msg kind => *)
-  (*     promise loc from to msg kind *)
-  (*   | silent => silent *)
-  (*   | read loc ts val released ord => *)
-  (*     read loc ts val released (Ordering.join ord0 ord) *)
-  (*   | write loc from to val released ord => *)
-  (*     write loc from to val released (Ordering.join ord0 ord) *)
-  (*   | update loc tsr tsw valr valw releasedr releasedw ordr ordw => *)
-  (*     update loc tsr tsw valr valw releasedr releasedw (Ordering.join ord0 ordr) (Ordering.join ord0 ordw) *)
-  (*   | fence ordr ordw => *)
-  (*     fence (Ordering.join ord0 ordr) (Ordering.join ord0 ordw) *)
-  (*   | syscall e => *)
-  (*     syscall e *)
-  (*   | failure => *)
-  (*     failure *)
-  (*   end. *)
-
-  (* Lemma lift_plain e: *)
-  (*   lift Ordering.plain e = e. *)
-  (* Proof. destruct e; ss. Qed. *)
 End ThreadEvent.
 
 Module Local.
@@ -277,7 +220,8 @@ Module Local.
   Hint Constructors read_step.
 
   Inductive write_step (lc1:t) (sc1:TimeMap.t) (mem1:Memory.t)
-                       (loc:Loc.t) (from to:Time.t) (val:Const.t) (releasedm released:option View.t) (ord:Ordering.t) (pf:bool)
+                       (loc:Loc.t) (from to:Time.t)
+                       (val:Const.t) (releasedm released:option View.t) (ord:Ordering.t)
                        (lc2:t) (sc2:TimeMap.t) (mem2:Memory.t) (kind:Memory.op_kind): Prop :=
   | write_step_intro
       promises2
@@ -285,10 +229,9 @@ Module Local.
       (WRITABLE: TView.writable lc1.(tview).(TView.cur) sc1 loc to ord)
       (WRITE: Memory.write lc1.(promises) mem1 loc from to val released promises2 mem2 kind)
       (RELEASE: Ordering.le Ordering.strong_relaxed ord -> Memory.nonsynch_loc loc lc1.(promises))
-      (PF: pf -> lc1.(promises) loc = Cell.bot)
       (LC2: lc2 = mk (TView.write_tview lc1.(tview) sc1 loc to ord) promises2)
       (SC2: sc2 = sc1):
-      write_step lc1 sc1 mem1 loc from to val releasedm released ord pf lc2 sc2 mem2 kind
+      write_step lc1 sc1 mem1 loc from to val releasedm released ord lc2 sc2 mem2 kind
   .
   Hint Constructors write_step.
 
@@ -320,17 +263,17 @@ Module Local.
       program_step (ThreadEvent.read loc ts val released ord) lc1 sc1 mem1 lc2 sc1 mem1
   | step_write
       lc1 sc1 mem1
-      loc from to val released ord pf lc2 sc2 mem2 kind
-      (LOCAL: Local.write_step lc1 sc1 mem1 loc from to val None released ord pf lc2 sc2 mem2 kind):
-      program_step (ThreadEvent.write loc from to val released ord pf) lc1 sc1 mem1 lc2 sc2 mem2
+      loc from to val released ord lc2 sc2 mem2 kind
+      (LOCAL: Local.write_step lc1 sc1 mem1 loc from to val None released ord lc2 sc2 mem2 kind):
+      program_step (ThreadEvent.write loc from to val released ord) lc1 sc1 mem1 lc2 sc2 mem2
   | step_update
       lc1 sc1 mem1
-      loc ordr ordw pf
+      loc ordr ordw
       tsr valr releasedr releasedw lc2
       tsw valw lc3 sc3 mem3 kind
       (LOCAL1: Local.read_step lc1 mem1 loc tsr valr releasedr ordr lc2)
-      (LOCAL2: Local.write_step lc2 sc1 mem1 loc tsr tsw valw releasedr releasedw ordw pf lc3 sc3 mem3 kind):
-      program_step (ThreadEvent.update loc tsr tsw valr valw releasedr releasedw ordr ordw pf)
+      (LOCAL2: Local.write_step lc2 sc1 mem1 loc tsr tsw valw releasedr releasedw ordw lc3 sc3 mem3 kind):
+      program_step (ThreadEvent.update loc tsr tsw valr valw releasedr releasedw ordr ordw)
                    lc1 sc1 mem1 lc3 sc3 mem3
   | step_fence
       lc1 sc1 mem1
@@ -401,8 +344,8 @@ Module Local.
   Qed.
 
   Lemma write_step_future
-        lc1 sc1 mem1 loc from to val releasedm released ord pf lc2 sc2 mem2 kind
-        (STEP: write_step lc1 sc1 mem1 loc from to val releasedm released ord pf lc2 sc2 mem2 kind)
+        lc1 sc1 mem1 loc from to val releasedm released ord lc2 sc2 mem2 kind
+        (STEP: write_step lc1 sc1 mem1 loc from to val releasedm released ord lc2 sc2 mem2 kind)
         (REL_WF: View.opt_wf releasedm)
         (REL_CLOSED: Memory.closed_opt_view releasedm mem1)
         (WF1: wf lc1 mem1)
@@ -431,17 +374,17 @@ Module Local.
   Qed.
 
   Lemma write_step_non_cancel
-        lc1 sc1 mem1 loc from to val releasedm released ord pf lc2 sc2 mem2 kind
-        (STEP: write_step lc1 sc1 mem1 loc from to val releasedm released ord pf lc2 sc2 mem2 kind):
+        lc1 sc1 mem1 loc from to val releasedm released ord lc2 sc2 mem2 kind
+        (STEP: write_step lc1 sc1 mem1 loc from to val releasedm released ord lc2 sc2 mem2 kind):
     negb (Memory.op_kind_is_cancel kind).
   Proof.
     inv STEP. inv WRITE. inv PROMISE; ss.
   Qed.
 
   Lemma write_step_strong_relaxed
-        lc1 sc1 mem1 loc from to val releasedm released ord pf lc2 sc2 mem2 kind
-        (STEP: write_step lc1 sc1 mem1 loc from to val releasedm released ord pf lc2 sc2 mem2 kind)
-        (ORD: Ordering.le Ordering.strong_relaxed ord \/ pf):
+        lc1 sc1 mem1 loc from to val releasedm released ord lc2 sc2 mem2 kind
+        (STEP: write_step lc1 sc1 mem1 loc from to val releasedm released ord lc2 sc2 mem2 kind)
+        (ORD: Ordering.le Ordering.strong_relaxed ord):
     negb (Memory.op_kind_is_lower kind).
   Proof.
     guardH ORD.
@@ -449,12 +392,9 @@ Module Local.
     inv PROMISE. des. subst.
     exploit Memory.lower_get0; try exact PROMISES. i. des.
     unguard. des.
-    - exploit RELEASE; eauto. inv MSG_LE; eauto. i. subst.
-      inv RELEASED. revert H0.
-      unfold TView.write_released. condtac; ss. destruct ord; ss.
-    - destruct pf; ss.
-      unfold Memory.get in *. rewrite PF in *; ss.
-      rewrite Cell.bot_get in *. ss.
+    exploit RELEASE; eauto. inv MSG_LE; eauto. i. subst.
+    inv RELEASED. revert H0.
+    unfold TView.write_released. condtac; ss. destruct ord; ss.
   Qed.
 
   Lemma fence_step_future
@@ -562,8 +502,8 @@ Module Local.
   Qed.
 
   Lemma write_step_disjoint
-        lc1 sc1 mem1 lc2 sc2 loc from to val releasedm released ord pf mem2 kind lc
-        (STEP: write_step lc1 sc1 mem1 loc from to val releasedm released ord pf lc2 sc2 mem2 kind)
+        lc1 sc1 mem1 lc2 sc2 loc from to val releasedm released ord mem2 kind lc
+        (STEP: write_step lc1 sc1 mem1 loc from to val releasedm released ord lc2 sc2 mem2 kind)
         (WF1: wf lc1 mem1)
         (SC1: Memory.closed_timemap sc1 mem1)
         (CLOSED1: Memory.closed mem1)
